\begin{uebung}
  Rechnen Sie nach:
  \begin{enumerate}
  \item
    \begin{align*}
      \nabla\cdot(\rho v) = \rho \nabla \cdot v + v \cdot \nabla \rho
    \end{align*}
\item
  \begin{align*}
    \nabla \cdot (\rho v \oplus v) = (v \oplus v) \nabla \rho + \rho (\nabla \cdot v )v + \rho (v \cdot \nabla)v.
  \end{align*}
  \end{enumerate}
\end{uebung}
\begin{uebung}
  Rechnen Sie nach:
  \begin{align*}
    - \Delta v = - \nabla \cdot \nabla v = - \nabla \nabla \cdot v + \nabla \times \nabla \times v.
  \end{align*}
\end{uebung}